theories/imports.v
@@ -8,10 +8,3 @@ Require Export Psatz.
 
 Global Set Warnings "-notation-overridden".
 Require Export Autosubst2.syntax.
-
-Notation "s [ sigmatm ]" := (subst_tm sigmatm s) (at level 7, left associativity) : subst_scope.
-Notation "s ⟨ xitm ⟩" := (ren_tm xitm s) (at level 7, left associativity) : subst_scope.
-
-Global Disable Notation "'var'" : subst_scope.
-Global Disable Notation "↑".
-Global Open Scope subst_scope. 
