gen_syntax.pl
@@ -1,0 +1,33 @@
+#!/usr/bin/env perl
+use strict;
+use warnings;
+use Path::Tiny;
+use utf8;
+
+my $prelude = <<'END_PRELUDE';
+Require Export Lattice.All.
+Require Export unscoped.
+
+Module Type syntax_sig
+  (Export lattice : Lattice).
+END_PRELUDE
+
+my $prologue = <<'END_PROLOGUE';
+
+Notation "s [ sigmatm ]" := (subst_tm sigmatm s) (at level 7, left associativity) : subst_scope.
+Notation "s ⟨ xitm ⟩" := (ren_tm xitm s) (at level 7, left associativity) : subst_scope.
+
+Global Disable Notation "'var'" : subst_scope.
+Global Disable Notation "↑".
+Global Open Scope subst_scope.
+
+End syntax_sig.
+END_PROLOGUE
+
+my $syntax_path = path('theories/Autosubst2/syntax.v');
+
+my $syntax = join('',map { (my $s = $_) =~ s/^(Hint|Instance)/#[export]$1/; $s } grep(!/^Require Export/,$syntax_path->lines_utf8));
+
+$syntax =~ s/\(\(fun \w+ => \(eq_refl\) \w+\) \w+\)/eq_refl/g;
+
+$syntax_path->spew_utf8($prelude,$syntax,$prologue);
